test/new_treehash/test_new_version.c
@@ -193,7 +193,7 @@ int main() {
     // char *impls[] = {"XMSS-SHA2_10_256", "XMSS-SHA2_10_192", "XMSSMT-SHA2_20/2_256", "XMSSMT-SHA2_20/4_256"};
     char *impls[] = {"XMSSMT-SHA2_20/2_256"};
 
-    size_t impl_count = 4;
+    size_t impl_count = 1; /* TODO: Update this */
 
     for (size_t i = 0; i < impl_count; i++) {
         if (starts_with(impls[i], "XMSSMT")) {
