proof/correctness/Correctness_WOTS.ec
@@ -156,7 +156,93 @@ lemma base_w_results_64 ( _in_ : W8.t Array32.t) :
       forall (k : int), 0 <= k < 64 => 0 <= to_uint res{1}.[k] < w
     ].
 proof.
-admit. (* correctness + bounds *)
+rewrite /XMSS_WOTS_W /XMSS_WOTS_LOG_W => [#] logw_val w_val.
+proc.
+sp.
+while (
+  ={total, consumed} /\ 0 <= consumed{1} <= 64 /\
+  size base_w{2} = 64 /\
+  outlen{2} = 64 /\
+  out{2} = to_uint out{1} /\
+  out{2} = consumed{1} /\
+  X{2} = to_list input{1} /\
+  out{2} = to_uint out{1} /\ 0 <= to_uint out{1} <= 67 /\
+  bits{2} = to_uint bits{1} /\ 
+  bits{2} = consumed{2} %% 2 * 4 /\
+  _in{2} = to_uint in_0{1} /\ _in{2} = (consumed{2} + 1) %/ 2 /\
+  (forall (j : int), 0 <= j < to_uint out{1} => (to_uint output{1}.[j]) = nth witness base_w{2} j) /\
+  (forall (j : int), 0 <= j < to_uint out{1} => 0 <= to_uint output{1}.[j] < w)
+); last first.
+    + auto => /> &1.
+      do split.
+         * by rewrite size_nseq.
+         * smt().
+         * smt().
+         * move => bitsL inL outL resultL resultR H0 H1 H2 H3 H4 H5 H6 H7 H8 H9 H10.
+           split => [| /#].
+           apply (eq_from_nth witness); first by rewrite H4 size_map size_to_list.
+           rewrite H4 => i?.
+           rewrite (nth_map witness). 
+              - by rewrite size_to_list.
+           rewrite get_to_list H9 //#.
+if.
+    + auto => /> &1 &2 *; smt(@W64).
+    + auto => /> &1 &2 H0 H1 H2 H3 H4 H5 H6 H7 H8 H9. 
+      do split.
+        * smt().
+        * smt().
+        * by rewrite size_put.
+        * rewrite to_uintD /#.
+        * rewrite to_uintD /#.
+        * rewrite to_uintD /#.
+        * rewrite to_uintD /#.
+        * by rewrite logw_val.
+        * rewrite logw_val /=/#.
+        * rewrite to_uintD /#.
+        * smt().
+        * rewrite to_uintD_small 1:/# /= => j??.
+          rewrite nth_put 1:/# get_setE //.
+          case (j = to_uint out{1}) => [-> |?]; last first.
+               - rewrite ifF 1:/# H7 //#.
+          rewrite w_val ifT // log2_16 from_int_floor /= (: 15 = 2 ^ 4 - 1) 1:/# !and_mod //.
+          rewrite (: 31 = 2 ^ 5 - 1) 1:/# !shr_div !of_uintK and_mod //=.
+          smt(modz_small).
+        * rewrite to_uintD_small 1:/# /= => j??.
+          rewrite (: 31 = 2 ^ 5 - 1) 1:/# !and_mod // of_uintK.
+          rewrite get_setE //.
+          case (j = to_uint out{1}) => [?| /#].
+          rewrite (: 15 = 2 ^ 4 - 1) 1:/# !and_mod // of_uintK.
+          smt(modz_small).
+    + auto => /> &1 &2 H0 H1 H2 H3 H4 H5 H6 H7 H8 H9 H10.
+      do split.
+        * smt().
+        * smt().
+        * by rewrite size_put.
+        * rewrite to_uintD /#.
+        * rewrite to_uintD /#.
+        * rewrite to_uintD /#.
+        * rewrite to_uintD /#.
+        * rewrite logw_val to_uintB // #smt:(@W64 pow2_64 modz_small).
+        * rewrite logw_val H5 /= #smt:(@W64 pow2_64 modz_small).
+        * rewrite H6 #smt:(@W64 pow2_64 @IntDiv).  
+        * rewrite to_uintD_small 1:/# /= => j??.
+          rewrite nth_put 1:/# get_setE //.
+          case (j = to_uint out{1}) => [-> |?]; last first.
+             - rewrite ifF 1:/# H7 //#.
+          rewrite ifT // logw_val w_val /= (: 15 = 2^4 - 1) 1:/# (: 31 = 2^5 - 1) 1:/# !and_mod // !of_uintK //=.
+          rewrite to_uint_shr.
+             - rewrite !of_uintK /#.
+          rewrite to_uint_shr.
+             - rewrite !of_uintK /#.
+         rewrite to_uint_truncateu8 to_uint_zeroextu32 !of_uintK /=. 
+         smt(@IntDiv @W64 pow2_64 modz_small).
+        * rewrite to_uintD_small 1:/# /= => j??. 
+          rewrite (: 31 = 2^5 - 1) 1:/# (: 15 = 2^4 - 1) 1:/# !and_mod //=.        
+          rewrite to_uint_shr.
+             - rewrite !of_uintK /#.
+          rewrite get_setE //.
+          case (j = to_uint out{1}) => [?| /#].
+          rewrite to_uint_zeroextu32 to_uint_truncateu8 !of_uintK #smt:(modz_small).
 qed.
 
 lemma base_w_correctness_3 ( _in_ : W8.t Array2.t) :
@@ -247,11 +333,96 @@ lemma base_w_results_3 ( _in_ : W8.t Array2.t) :
       arg{2} = (to_list _in_, 3) 
       ==>
       res{2} = map (W32.to_uint) (to_list res{1}) /\
-        forall (x : int), x \in res{2} => 0 <= x < w
+      forall (k : int), 0 <= k < 3 => 0 <= to_uint res{1}.[k] < w
     ].
 proof.
-move => [#] ??. 
-admit.
+rewrite /XMSS_WOTS_W /XMSS_WOTS_LOG_W => [#] logw_val w_val.
+proc.
+sp.
+while (
+  ={total, consumed} /\ 0 <= consumed{1} <= 3 /\
+  size base_w{2} = 3 /\
+  outlen{2} = 3 /\
+  out{2} = to_uint out{1} /\
+  out{2} = consumed{1} /\
+  X{2} = to_list input{1} /\
+  out{2} = to_uint out{1} /\ 0 <= to_uint out{1} <= 67 /\
+  bits{2} = to_uint bits{1} /\ 
+  bits{2} = consumed{2} %% 2 * 4 /\
+  _in{2} = to_uint in_0{1} /\ _in{2} = (consumed{2} + 1) %/ 2 /\
+  (forall (j : int), 0 <= j < to_uint out{1} => (to_uint output{1}.[j]) = nth witness base_w{2} j) /\
+  (forall (j : int), 0 <= j < to_uint out{1} => 0 <= to_uint output{1}.[j] < w)
+); last first.
+    + auto => /> &1.
+      do split.
+         * by rewrite size_nseq.
+         * smt().
+         * smt().
+         * move => bitsL inL outL resultL resultR H0 H1 H2 H3 H4 H5 H6 H7 H8 H9 H10.
+           split => [| /#].
+           apply (eq_from_nth witness); first by rewrite H4 size_map size_to_list.
+           rewrite H4 => i?.
+           rewrite (nth_map witness). 
+              - by rewrite size_to_list.
+           rewrite get_to_list H9 //#.
+if.
+    + auto => /> &1 &2 *; smt(@W64).
+    + auto => /> &1 &2 H0 H1 H2 H3 H4 H5 H6 H7 H8 H9. 
+      do split.
+        * smt().
+        * smt().
+        * by rewrite size_put.
+        * rewrite to_uintD /#.
+        * rewrite to_uintD /#.
+        * rewrite to_uintD /#.
+        * rewrite to_uintD /#.
+        * by rewrite logw_val.
+        * rewrite logw_val /=/#.
+        * rewrite to_uintD /#.
+        * smt().
+        * rewrite to_uintD_small 1:/# /= => j??.
+          rewrite nth_put 1:/# get_setE //.
+          case (j = to_uint out{1}) => [-> |?]; last first.
+               - rewrite ifF 1:/# H7 //#.
+          rewrite w_val ifT // log2_16 from_int_floor /= (: 15 = 2 ^ 4 - 1) 1:/# !and_mod //.
+          rewrite (: 31 = 2 ^ 5 - 1) 1:/# !shr_div !of_uintK and_mod //=.
+          smt(modz_small).
+        * rewrite to_uintD_small 1:/# /= => j??.
+          rewrite (: 31 = 2 ^ 5 - 1) 1:/# !and_mod // of_uintK.
+          rewrite get_setE //.
+          case (j = to_uint out{1}) => [?| /#].
+          rewrite (: 15 = 2 ^ 4 - 1) 1:/# !and_mod // of_uintK.
+          smt(modz_small).
+    + auto => /> &1 &2 H0 H1 H2 H3 H4 H5 H6 H7 H8 H9 H10.
+      do split.
+        * smt().
+        * smt().
+        * by rewrite size_put.
+        * rewrite to_uintD /#.
+        * rewrite to_uintD /#.
+        * rewrite to_uintD /#.
+        * rewrite to_uintD /#.
+        * rewrite logw_val to_uintB // #smt:(@W64 pow2_3 modz_small).
+        * rewrite logw_val H5 //= #smt:(@W64 pow2_32 modz_small @IntDiv).
+        * rewrite H6 #smt:(@W64 pow2_32 @IntDiv).  
+        * rewrite to_uintD_small 1:/# /= => j??.
+          rewrite nth_put 1:/# get_setE //.
+          case (j = to_uint out{1}) => [-> |?]; last first.
+             - rewrite ifF 1:/# H7 //#.
+          rewrite ifT // logw_val w_val /= (: 15 = 2^4 - 1) 1:/# (: 31 = 2^5 - 1) 1:/# !and_mod // !of_uintK //=.
+          rewrite to_uint_shr.
+             - rewrite !of_uintK /#.
+          rewrite to_uint_shr.
+             - rewrite !of_uintK /#.
+         rewrite to_uint_truncateu8 to_uint_zeroextu32 !of_uintK /=. 
+         smt(@IntDiv @W64 modz_small).
+        * rewrite to_uintD_small 1:/# /= => j??. 
+          rewrite (: 31 = 2^5 - 1) 1:/# (: 15 = 2^4 - 1) 1:/# !and_mod //=.        
+          rewrite to_uint_shr.
+             - rewrite !of_uintK /#.
+          rewrite get_setE //.
+          case (j = to_uint out{1}) => [?| /#].
+          rewrite to_uint_zeroextu32 to_uint_truncateu8 !of_uintK #smt:(modz_small).
 qed.
 
 lemma wots_checksum_correctness (msg : W32.t Array64.t) :
@@ -290,10 +461,36 @@ lemma wots_checksum_results (msg : W32.t Array64.t) :
       arg{1} = msg /\ arg{2} = map (W32.to_uint) (to_list msg) 
       ==>
       to_uint res{1} = res{2} /\
-        0 <= res{2} <= len1 * (w - 1) 
+      0 <= res{2} <= len1 * (w - 1) 
     ].
 proof.
-admit.
+rewrite /XMSS_WOTS_LEN1 /XMSS_WOTS_W => [#] len1_val w_val.
+proc => /=.
+while (
+  #pre /\
+  to_uint csum{1} = checksum{2} /\
+  0 <= to_uint csum{1} <= (i{2} * (w - 1) * 2^8) /\
+  i{2} = to_uint i{1} /\ 
+  0 <= i{2} <= len1 /\
+  m{2} = map (W32.to_uint) (to_list msg{1}) /\
+  0 <= checksum{2} <= i{2} * (w - 1)
+); last by auto => /> /#.
+    + auto => /> &1 &2 H0 H1 H2 H3 H4 H5 H6.
+      do split.
+        * rewrite (nth_map witness); first by rewrite size_to_list /#.
+          rewrite get_to_list w_val /= to_uintD to_uintB.
+            - rewrite uleE of_uintK /= /#.
+          rewrite of_uintK /= to_uint_zeroextu64 /#.
+        * rewrite !to_uintD to_uintN to_uint_zeroextu64 of_uintK /= /#.
+        * rewrite !to_uintD of_uintK /= to_uintN to_uint_zeroextu64 /#.
+        * rewrite to_uintD /#.
+        * smt().
+        * smt().
+        * rewrite (nth_map witness); first by rewrite size_to_list /#.
+          rewrite get_to_list /#.
+        * rewrite (nth_map witness); [by rewrite size_to_list /#|] => /#.
+        * rewrite ultE of_uintK /= to_uintD /#.
+        * rewrite ultE of_uintK to_uintD /#.
 qed.
 
 lemma gen_chain_inplace_correct (_buf_ : W8.t Array32.t, _start_ _steps_ : W32.t, _addr_ : W32.t Array8.t, _pub_seed_ : W8.t Array32.t) :
@@ -627,23 +824,6 @@ case (i{2} * 32 <= k && k < i{2} * 32 + 32) => *.
       apply H2 => /#.
 qed.
 
-lemma expand_seed_results (_in_seed _pub_seed : W8.t Array32.t, _addr : W32.t Array8.t) :
-    len = XMSS_WOTS_LEN /\ 
-    n = XMSS_N /\ 
-    prf_padding_val = XMSS_HASH_PADDING_PRF /\
-    prf_kg_padding_val = XMSS_HASH_PADDING_PRF_KEYGEN /\
-    padding_len = XMSS_PADDING_LEN =>
-    equiv [M(Syscall).__expand_seed ~ WOTS.pseudorandom_genSK :
-      arg{1}.`2 = _in_seed /\ 
-      arg{1}.`3 = _pub_seed /\
-      arg{1}.`4 = _addr /\
-      arg{2} = (NBytes.insubd (to_list _in_seed), NBytes.insubd (to_list _pub_seed), _addr) ==>
-      res{1}.`1 = DecodeWotsSk res{2}
-    ].
-proof.
-admit. (* correctness & wots_sk_size from properties *)
-qed.
-
 lemma pkgen_correct (_seed_ _pub_seed_ : W8.t Array32.t) :
     w = XMSS_WOTS_W /\
     len = XMSS_WOTS_LEN /\
@@ -688,7 +868,7 @@ seq 1 1: (
       skip => /> &1 &2 *; do split.
           * by rewrite insubdK // /P size_to_list n_val.
           * by rewrite insubdK // /P size_to_list n_val.
-          * admit. (* expand_Seed needs information about the result *)
+          * admit. (* expand_Seed needs information about the address in the result *)
 conseq (: _ ==> 
   address{2} = addr{1} /\ 
   size pk{2} = len /\
@@ -773,8 +953,43 @@ move => k??.
 rewrite /DecodeWotsSk /of_list initiE 1:/# => />.
 qed.
 
-(*** Pk From Sig : Doing ***)
 
+lemma pkgen_results (_seed_ _pub_seed_ : W8.t Array32.t) (a1 a2 : adrs) :
+    w = XMSS_WOTS_W /\
+    len = XMSS_WOTS_LEN /\
+    n = XMSS_N /\
+    prf_padding_val = XMSS_HASH_PADDING_PRF /\
+    prf_kg_padding_val = XMSS_HASH_PADDING_PRF_KEYGEN /\
+    padding_len = XMSS_PADDING_LEN /\
+    F_padding_val = XMSS_HASH_PADDING_F =>
+    equiv [
+      M(Syscall).__wots_pkgen ~ WOTS.pkGen :
+      arg{1}.`2 = _seed_ /\
+      arg{1}.`3 = _pub_seed_ /\
+      arg{1}.`4 = a1 /\
+
+      arg{2}.`1 = NBytes.insubd (to_list _seed_) /\
+      arg{2}.`2 = NBytes.insubd (to_list _pub_seed_) /\
+      arg{2}.`3 = a2 /\
+
+      forall (k : int), 0 <= k < 5 => a1.[k] = a2.[k]
+
+      ==>
+
+      res{1}.`1 = DecodeWotsPk res{2} /\
+      forall (k : int), 0 <= k < 5 => res{1}.`2.[k] = a1.[k]
+    ]. 
+proof.
+rewrite /XMSS_WOTS_W /XMSS_WOTS_LEN /XMSS_N /XMSS_HASH_PADDING_PRF.
+rewrite /XMSS_HASH_PADDING_PRF_KEYGEN /XMSS_PADDING_LEN /XMSS_HASH_PADDING_F.
+move => [#] w_val len_val n_val *.
+proc.
+admit.
+qed.
+
+
+
+(*** Pk From Sig : Doing ***)
 
 lemma pk_from_sig_correct (mem : global_mem_t) (_sig_ptr_ : W64.t, _msg_ _pub_seed_ : W8.t Array32.t, _addr_ : W32.t Array8.t) :
     valid_ptr_i _sig_ptr_ 2144 =>
