proof/correctness/TreehashProof.ec
@@ -13,23 +13,49 @@ require import Params XMSS_MT_Params Types XMSS_MT_Types Address Hash BaseW WOTS
 require import XMSS_IMPL Parameters.
 require import Repr2 Utils2.
 
-require import Array4 Array8 Array11 Array32 Array131 Array320 Array352 Array2144 Array2464.
+require import Array4 Array8 Array11 Array32 Array64 Array131 Array320 Array352 Array2144 Array2464.
 
 require import Correctness_Address.
 require import Correctness_WOTS.
+require import Correctness_Hash.
 require import Correctness_Mem.
 require import Correctness_Conditions.
-(* require import LTReeProof. *)
+require import LTReeProof.
 
 require import WArray32.
 
-(* 
-{1} => proc __treehash (root:W8.t Array32.t, sk_seed:W8.t Array32.t,
-                   pub_seed:W8.t Array32.t, start_index:W32.t,
-                   target_height:W32.t, subtree_addr:W32.t Array8.t)
+lemma nth_nbytes_flatten (x : nbytes list, i : int):
+    0 <= i %/ n < size x =>
+    nth witness (nbytes_flatten x) i = nth witness (val (nth witness x (i %/ n))) (i %% n).
+move => H.
+rewrite /nbytes_flatten (nth_flatten witness n).
+    - pose P := (fun (s0 : W8.t list) => size s0 = n).
+      pose L := (map NBytes.val x).
+      rewrite -(all_nthP P L witness) /P /L size_map => j?. 
+      by rewrite (nth_map witness) // valP.
+by rewrite (nth_map witness).
+qed.
 
-{2} => proc treehash(pub_seed sk_seed : seed, s t : int, address : adrs) : nbytes
-*)
+lemma to_uint_eq_int_W32 (a b : W32.t) :
+    0 <= to_uint a < W32.max_uint =>
+    0 <= to_uint b < W32.max_uint =>
+    to_uint a = to_uint b =>
+    a = b by smt(@W32 pow2_32).
+
+(* Se duas slices sao iguais, duas slices dessas slices tb sao *)
+lemma sub_N (a1 a2: W32.t Array8.t) (len1 len2 : int) :
+    0 <= len1 <= len2 =>
+    sub a1 0 len2 = sub a2 0 len2 =>
+    sub a1 0 len1 = sub a2 0 len1.
+proof.
+move => [H0 H1] H2.
+apply (eq_from_nth witness); first by rewrite !size_sub /#.
+rewrite size_sub // => i?.
+have ?: forall (k : int), 0 <= k < len2 => a1.[k] = a2.[k] by smt(sub_k).
+rewrite !nth_sub /#.
+qed.
+ 
+
 lemma treehash_correct ( _sk_seed _pub_seed : W8.t Array32.t, _s _t:W32.t, _addr:W32.t Array8.t): 
     n = XMSS_N /\
     d = XMSS_D /\
@@ -58,19 +84,80 @@ lemma treehash_correct ( _sk_seed _pub_seed : W8.t Array32.t, _s _t:W32.t, _addr
       arg{2}.`5 = _addr /\
 
       0 <= to_uint _t <= h /\
-      0 <= to_uint _s <= to_uint _t
+      0 <= to_uint _s <= to_uint _t /\
+      _addr.[4] = W32.zero
       ==>
       to_list res{1} = val res{2}
     ]. 
-proof.
-rewrite /XMSS_N /XMSS_D /XMSS_TREE_HEIGHT /XMSS_FULL_HEIGHT /XMSS_D /= => [#] n_val d_val h_val tree_height *.
+proof. 
+rewrite /XMSS_N /XMSS_D /XMSS_TREE_HEIGHT /XMSS_FULL_HEIGHT /XMSS_D /XMSS_WOTS_W /XMSS_WOTS_LEN /= .
+move => [#] n_val d_val h_val tree_height *.
+rewrite h_val d_val in tree_height. 
 proc => /=.
- 
-swap {2} 3 -2.
-seq 8 1: (#pre /\ offset{1} = W64.zero /\ offset{2} = 0); first by auto.
+have E0 : 2 ^ h = 1048576 by rewrite h_val /#.
+seq 7 0 : #pre; first by auto. 
+seq 4 3 : (
+  #pre /\
+  offset{1} = W64.zero /\
+  offset{2} = to_uint offset{1} /\
+  ots_addr{1} = subtree_addr{1} /\
+  ltree_addr{1} = subtree_addr{1} /\
+  node_addr{1} = subtree_addr{1} /\
+  node_addr{1}.[4] = W32.zero /\
+  address{2}.[4] = W32.zero /\
 
-seq 11 4 : (sub _stack{1} 0 n = val (nth witness stack{2} 0)); last first.
-  + while {1}
+  size stack{2} = h %/ d + 1 /\ (* = 11 *)
+  size heights{2} = h %/ d + 1  /\   (* = 11 *)
+  size stack{2} = size heights{2}
+).
+    + auto => /> ???? H; do split; 5,6: by rewrite size_nseq /#.
+         * rewrite tP => j*.
+           rewrite initiE //= get32E pack4E wordP => i?.
+           rewrite initiE //= initiE 1:/# /= /init64 initiE 1:/# /= /copy_64 initiE 1:/# /=.
+           rewrite  get64E pack8E bits8iE 1:/# initiE 1:/# /= initiE 1:/# //= /init32 initiE 1:/# /= bits8iE /#.
+         * rewrite tP => j*.
+           rewrite initiE //= get32E pack4E wordP => i?.
+           rewrite initiE //= initiE 1:/# /= /init64 initiE 1:/# /= /copy_64 initiE 1:/# /=.
+           rewrite  get64E pack8E bits8iE 1:/# initiE 1:/# /= initiE 1:/# //= /init32 initiE 1:/# /= bits8iE /#.
+         * rewrite tP => j*.
+           rewrite initiE //= get32E pack4E wordP => i?.
+           rewrite initiE //= initiE 1:/# /= /init64 initiE 1:/# /= /copy_64 initiE 1:/# /=.
+           rewrite  get64E pack8E bits8iE 1:/# initiE 1:/# /= initiE 1:/# //= /init32 initiE 1:/# /= bits8iE /#.
+         * rewrite /get32_direct pack4E wordP => i?.
+           rewrite initiE //= initiE 1:/# /= /init64 initiE 1:/# /= /copy_64 initiE 1:/# /=.
+           rewrite  get64E pack8E bits8iE 1:/# initiE 1:/# /= initiE 1:/# //= /init32 initiE 1:/# /= bits8iE 1:/#.
+           rewrite (: (8 * ((16 + i %/ 8) %/ 8) + ((16 + i %/ 8) %% 8 * 8 + i %% 8) %/ 8) %/ 4 = 4) 1:/# H /#.
+         * by rewrite !size_nseq. 
+
+seq 4 0 : (
+  #{/~ots_addr{1} = subtree_addr{1}}
+   {/~ltree_addr{1} = subtree_addr{1}}
+   {/~node_addr{1} = subtree_addr{1}}pre /\
+   sub ots_addr{1} 0 3 = sub address{2} 0 3 /\    (* coincidem nos indices 0, 1 e 2 *)
+   sub ltree_addr{1} 0 3 = sub address{2} 0 3 /\
+   sub node_addr{1} 0 3 = sub address{2} 0 3 /\
+   ots_addr{1}.[3] = W32.zero /\
+   ltree_addr{1}.[3] = W32.one /\
+   node_addr{1}.[3] = W32.of_int 2 /\
+   node_addr{1}.[4] = W32.zero
+).
+    + inline {1}.
+      auto => /> *.
+      do split; (
+          apply (eq_from_nth witness); [by rewrite !size_sub | rewrite size_sub // => ??]; 
+          by rewrite !nth_sub //= get_setE // ifF 1:/# 
+      ).
+
+swap {1} 1 2.
+
+seq 2 0 : (#pre /\ to_uint upper_bound{1} = 2^t{2}).
+    + auto => /> &2 *.
+      rewrite (: 31 = 2^5 - 1) 1:/# and_mod // shl_shlw 1:#smt:(@W32) of_uintK to_uint_shl 1:/# /=.
+      have ->: to_uint _t %% 32 %% 4294967296 = to_uint _t by smt(modz_small). 
+      smt(@IntDiv @RealExp).
+
+seq 2 2 : (sub _stack{1} 0 n = val (nth witness stack{2} 0)); last first.
+    + while {1}
     (#pre /\
      0 <= j{1} <= 32 /\ 
      node{2} = nth witness stack{2} 0 /\
@@ -89,680 +176,506 @@ seq 11 4 : (sub _stack{1} 0 n = val (nth witness stack{2} 0)); last first.
           rewrite -get_to_list -H0.
           by rewrite nth_sub 1:/# get_to_list.
 
-seq 0 2 : (#pre /\ size stack{2} = (h %/d + 1) /\ size heights{2} = (h %/ d)).
-      + auto => /> *; rewrite !size_nseq /#.
+while (
+      t{2} = to_uint target_height{1} /\ 0 <= t{2} <= h /\ (* Target height *)
+      s{2} = to_uint start_index{1} /\ 0 <= s{2} <= h /\ (* start index  *) 
 
-seq 1 0 : (#pre /\ ots_addr{1} = subtree_addr{1}).
-      + auto => /> *.
-        rewrite tP => j?.
-        rewrite initiE //= get32E pack4E wordP => i?.
-        rewrite initiE //= initiE 1:/# /= /init64 initiE 1:/# /= /copy_64 initiE 1:/# /=.
-        rewrite  get64E pack8E bits8iE 1:/# initiE 1:/# /= initiE 1:/# //= /init32 initiE 1:/# /= bits8iE /#.
+      0 <= offset{2} < size heights{2} /\ offset{2} = to_uint offset{1} /\  
+      (i{2} <> 0 => 0 < offset{2}) /\
 
-seq 1 0 : (#pre /\ ltree_addr{1} = subtree_addr{1}).
-      + auto => /> ??.
-        rewrite tP => j*.
-        rewrite initiE //= get32E pack4E wordP => i?.
-        rewrite initiE //= initiE 1:/# /= /init64 initiE 1:/# /= /copy_64 initiE 1:/# /=.
-        rewrite  get64E pack8E bits8iE 1:/# initiE 1:/# /= initiE 1:/# //= /init32 initiE 1:/# /= bits8iE /#.
+      0 <= i{2} <= 2^t{2} /\ to_uint i{1} = i{2} /\
+      to_uint upper_bound{1} = 2 ^ t{2} /\
 
-seq 1 0 : (#pre /\ node_addr{1} = subtree_addr{1}).
-      + auto => /> ??.
-        rewrite tP => j*.
-        rewrite initiE //= get32E pack4E wordP => i?.
-        rewrite initiE //= initiE 1:/# /= /init64 initiE 1:/# /= /copy_64 initiE 1:/# /=.
-        rewrite  get64E pack8E bits8iE 1:/# initiE 1:/# /= initiE 1:/# //= /init32 initiE 1:/# /= bits8iE /#.
+      size stack{2} = h %/ d + 1 /\ 
+      size heights{2} = h %/ d + 1 /\
 
-seq 4 0 : (
-      #{/~ ots_addr{1} = subtree_addr{1}}
-       {/~ ltree_addr{1} = subtree_addr{1}}
-       {/~ node_addr{1} = subtree_addr{1}}pre /\
-      ots_addr{1} = set_type subtree_addr{1} 0 /\
-      ltree_addr{1} = set_type subtree_addr{1} 1 /\
-      node_addr{1} = set_type subtree_addr{1} 2
-); first by inline; auto.
+      sk_seed{2} = (insubd (to_list sk_seed{1}))%NBytes /\
+      pub_seed{2} = (insubd (to_list pub_seed{1}))%NBytes /\ 
+      
+      sub ots_addr{1} 0 3 = sub address{2} 0 3 /\
+      sub ltree_addr{1} 0 3 = sub address{2} 0 3 /\
+      sub node_addr{1} 0 3 = sub address{2} 0 3 /\
 
-swap {1} 1 2.
+      ots_addr{1}.[3] = W32.zero /\       (* type *)
+      ltree_addr{1}.[3] = W32.one /\      (* type *)
+      node_addr{1}.[3] = W32.of_int 2 /\  (* type *)
+      node_addr{1}.[4] = W32.zero /\      (* padding *)
+      
+      map W32.to_uint (sub heights{1} 0 offset{2}) = sub_list heights{2} 0 offset{2} /\
+      (forall (k : int), 0 <= k < offset{2} => 0 <= nth witness heights{2} k < XMSS_TREE_HEIGHT) /\ 
 
-seq 2 0 : (#pre /\ to_uint upper_bound{1} = 2^t{2}).
-    + auto => /> &2. 
-      rewrite d_val h_val /= => *.
-      rewrite (: 31 = 2^5 - 1) 1:/# and_mod // shl_shlw 1:#smt:(@W32) of_uintK to_uint_shl 1:/# /=.
-      have ->: to_uint _t %% 32 %% 4294967296 = to_uint _t by smt(modz_small).
-      have E: 0 <= 2 ^ h < 4294967296 by rewrite h_val /#.
-      smt(@IntDiv @RealExp).
+      sub _stack{1} 0 (n * offset{2}) = sub_list (nbytes_flatten stack{2}) 0 (n * offset{2})
+); last first.
++ auto => /> &1 &2 H0 H1 H2 H3 H4 H5 H6 H7 H8 H9 H10 H11 H12 H13 H14 *.
+  rewrite pow2_nonnegative //.
+  do split; 1..2,4: by smt().
+        - apply (eq_from_nth witness); first by rewrite size_map size_sub // size_sub_list.
+          rewrite size_map size_sub /#.
+        - apply (eq_from_nth witness); first by rewrite size_sub // size_sub_list.
+          rewrite size_sub /#.
+        - rewrite ultE /#.
+        - rewrite ultE /#.
+        - move => _stack_L heights_L i_L ltree_addr_L node_add_L offset_L ots_addr_L address_R heights_R stack_R.
+          rewrite ultE => H15 H16 H17 H18 H19 H20 H21 H22 H23 H24 H25 H26 H27 H28 H29 H30 H31 H32 H33 H34.
+          apply (eq_from_nth witness); first by rewrite size_sub 1:/# valP n_val.
+          rewrite size_sub 1:/# n_val => j?.
+          have ?: 0 < to_uint i_L by smt(pow2_neq_0).
+          have := H34.
+          rewrite /sub /sub_list n_val.
+          have ->: 32 * to_uint offset_L = 32 + 32 * (to_uint offset_L - 1) by smt().
+          rewrite !(mkseq_add _ 32) 1..4:/# => H.
+          have ->: mkseq (fun (i0 : int) => _stack_L.[0 + i0]) 32 = mkseq (fun (i0 : int) => nth witness (nbytes_flatten stack_R) (0 + i0)) 32.
+             * have := eqseq_cat (mkseq (fun (i0 : int) => _stack_L.[0 + i0]) 32)
+               (mkseq (fun (i0 : int) => nth witness (nbytes_flatten stack_R) (0 + i0)) 32) (* 1st argument *)
+               (mkseq (fun (i0 : int) => (fun (i1 : int) => _stack_L.[0 + i1]) (32 + i0)) (32 * (to_uint offset_L - 1))) (* 2nd argument *)
+               (mkseq (fun (i0 : int) => (fun (i1 : int) => nth witness (nbytes_flatten stack_R) (0 + i1)) (32 + i0)) (32 * (to_uint offset_L - 1))) (* 3rd argument *).
+               by rewrite !size_mkseq /max //= H //=. 
+          rewrite nth_mkseq //= nth_nbytes_flatten /#.
 
-(* Rewrite #pre *)
-conseq (:
-  size stack{2} = h %/ d + 1 /\ 
-  size heights{2} = h %/ d /\
-
-  pub_seed{2} = (insubd (to_list pub_seed{1}))%NBytes /\
-  sk_seed{2} = (insubd (to_list sk_seed{1}))%NBytes /\
-  
-  address{2} = subtree_addr{1} /\
-
-  ots_addr{1} = set_type address{2} 0 /\
-  ltree_addr{1} = set_type address{2} 1 /\
-  node_addr{1} = set_type address{2} 2 /\
-  subtree_addr{1} = address{2} /\
-
-  ots_addr{1}.[3] = W32.zero /\
-  ltree_addr{1}.[3] = W32.one /\
-  node_addr{1}.[3] = W32.of_int 2 /\
-
-  offset{2} = to_uint offset{1} /\ 
-  offset{1} = W64.zero /\
-
-  t{2} = to_uint target_height{1} /\ 
-  0 <= t{2} <= h /\
-
-  s{2} = to_uint start_index{1} /\
-  0 <= s{2} <= t{2} /\
-
-  size stack{2} = h %/ d + 1 /\ 
-  size heights{2} = h %/ d /\
-
-  to_uint upper_bound{1} = 2^t{2}
-  ==> 
-  _
-); first by auto.
-
-(*
-
-=> The stack contains nodes at varying heights, with the height of each node stored in the heights array at the corresponding offset.
-
-=> When two nodes on the stack are at the same height, they are combined (& removed from the stack), and the resulting node is pushed onto the stack 
-
-=> No fim, offset = 1 (esta um nodo na stack 
-*) 
- 
-while ( 
-  t{2} = to_uint target_height{1} /\ 
-  0 <= t{2} <= h /\ (* Target height *)
-
-  s{2} = to_uint start_index{1} /\ 
-  0 <= s{2} <= h /\ (* start index  *) 
-
-  offset{2} = to_uint offset{1} /\  
-
-  (i{2} <> 0 => 0 < offset{2}) /\
-
-  0 <= offset{2} <= size stack{2} /\
-
-  size stack{2} = h %/ d + 1 /\ 
-  size heights{2} = h %/ d /\
-
-  0 <= i{2} <= 2^t{2} /\
-  i{2} <= to_uint target_height{1} /\
-  to_uint i{1} = i{2} /\
-
-  to_uint upper_bound{1} = 2^t{2} /\
-
-  sk_seed{2} = (insubd (to_list sk_seed{1}))%NBytes /\
-  pub_seed{2} = (insubd (to_list pub_seed{1}))%NBytes /\ 
-
-  map W32.to_uint (sub heights{1} 0 offset{2}) = sub_list heights{2} 0 offset{2} /\
-  sub _stack{1} 0 (n * offset{2}) = sub_list (nbytes_flatten stack{2}) 0 (n * offset{2}) /\
-
-  ots_addr{1}.[3] = W32.zero /\
-  ltree_addr{1}.[3] = W32.one /\
-  node_addr{1}.[3] = W32.of_int 2 /\
-
-  sub ots_addr{1} 0 3 = sub address{2} 0 3 /\ 
-  sub ltree_addr{1} 0 3 = sub address{2} 0 3 
-); first by admit.
-    + auto => /> &1 &2 *; do split.
-        * smt(@W32 pow2_32).
-        * smt(pow2_neq_0).
-        * smt(pow2_nonnegative).
-        * apply (eq_from_nth witness); first by rewrite size_map size_sub_list // size_sub.
-          rewrite size_map size_sub // /#.
-        * apply (eq_from_nth witness); first by rewrite size_sub // size_sub_list.
-          rewrite size_sub // /#.
-        * apply (eq_from_nth witness); first by rewrite !size_sub.
-          rewrite size_sub // => j?. 
-          by rewrite !nth_sub //= /set_type get_setE // ifF 1:/#.
-        * apply (eq_from_nth witness); first by rewrite !size_sub.
-          rewrite size_sub // => j?. 
-          by rewrite !nth_sub //= /set_type get_setE // ifF 1:/#.
-        * rewrite ultE /#.
-        * rewrite ultE /#. 
-
-        * move => stackImpl heightsImpl i ltree_addr heightSpec offsetImpl ots_addr addrSpec heightsSpec stackSpec.
-          rewrite ultE => ????????????H2*. 
-          have ?: 0 < to_uint i by smt(pow2_neq_0).
-          move: H2.
-          rewrite /sub n_val.
-          have ->: 32 * to_uint offsetImpl = 32 + 32 * (to_uint offsetImpl - 1) by smt().
-          rewrite /sub_list !(mkseq_add _ 32) 1..4:/# => H.
-          have ->: mkseq (fun (i0 : int) => stackImpl.[0 + i0]) 32 = mkseq (fun (i0 : int) => nth witness (nbytes_flatten stackSpec) (0 + i0)) 32.
-               + have := eqseq_cat (mkseq (fun (i0 : int) => stackImpl.[0 + i0]) 32)
-                (mkseq (fun (i0 : int) => nth witness (nbytes_flatten stackSpec) (0 + i0)) 32) (* 1st argument *)
-                (mkseq (fun (i0 : int) => (fun (i1 : int) => stackImpl.[0 + i1]) (32 + i0)) (32 * (to_uint offsetImpl - 1))) (* 2nd argument *)
-                (mkseq (fun (i0 : int) => (fun (i1 : int) => nth witness (nbytes_flatten stackSpec) (0 + i1)) (32 + i0)) (32 * (to_uint offsetImpl - 1))). (* 3rd argument *)
-                by rewrite !size_mkseq /max //= H //=. 
-          apply (eq_from_nth witness); first by rewrite size_mkseq valP /#.
-          rewrite size_mkseq => j?.
-          rewrite nth_mkseq //= /nbytes_flatten (nth_flatten witness n).
-            + pose P := (fun (s0 : W8.t list) => size s0 = n).
-              pose L := (map NBytes.val stackSpec).
-              rewrite -(all_nthP P L witness) /P /L size_map.
-              rewrite (: size stackSpec = h %/ d + 1) 1:/#.
-              rewrite d_val h_val /= => k?. 
-              by rewrite (nth_map witness) 1:/# valP. 
-          by rewrite (nth_map witness) /#.
- 
-(*================ O ultimo goal do while termina aqui ====================== *)
- 
 seq 2 0 : (#pre /\ to_uint t32{1} = s{2} + i{2}).
     + auto => /> &1 &2 *.
-      rewrite to_uintD_small //= /#.
+      rewrite to_uintD_small //=. 
+      smt(@IntDiv @RealExp).
+ 
+swap {1} 2 -1.
+
+seq 1 2 : (
+    #{/~sub ots_addr{1} 0 3 = sub address{2} 0 3}pre /\ sub ots_addr{1} 0 5 = sub address{2} 0 5
+).
+    + inline {1}; auto => /> &1 &2 H0 H1 H2 H3 H4 H5 H6 H7 H8 H9 H10 H11 H12 H13 H14 H15 H16 H17 H18 H19 H20 H21 H22 H23 H24. 
+      rewrite /set_ots_addr /set_type.
+      do split; (
+         apply (eq_from_nth witness); [by rewrite !size_sub | rewrite size_sub // => j?];
+         rewrite !nth_sub //= !get_setE //
+      ).
+         * do (rewrite ifF 1:/#).
+           have ->: ltree_addr{1}.[j] = nth witness (sub ltree_addr{1} 0 3) j by rewrite nth_sub.
+           by rewrite H13 nth_sub.
+         * do (rewrite ifF 1:/#).
+           have ->: node_addr{1}.[j] = nth witness (sub node_addr{1} 0 3) j by rewrite nth_sub.
+           by rewrite H14 nth_sub.
+         * case (j = 4) => ?.
+              - smt(@W32 pow2_32).
+              - do 3! (rewrite ifF 1:/#).
+                case (j = 3) => [/# |?].
+                have ->: ots_addr{1}.[j] = nth witness (sub ots_addr{1} 0 3) j by rewrite nth_sub /#.
+                rewrite H12 nth_sub /#.
 
 wp.
 
-seq 1 0 : (#pre /\ to_uint ltree_addr{1}.[4] = s{2} + i{2}).
-    + inline {1}; auto => /> &1 &2 ???????????????????<- *. 
-      (* A seta refere se a hipotese sub ltree_addr{1} 0 3 = sub address{2} 0 3 *)
-      apply (eq_from_nth witness); first by rewrite !size_sub.
-      rewrite size_sub // => j?.
-      by rewrite !nth_sub //= get_setE // ifF 1:/#. 
+seq 1 0 : (#pre /\ ltree_addr{1}.[4] = W32.of_int (s{2} + i{2})).
+    + inline {1}; auto => /> &1 &2 H0 H1 H2 H3 H4 H5 H6 H7 H8 H9 H10 H11 H12 H13 H14 H15 H16 H17 H18 H19 H20 H21 H22 H23 H24 *.
+      split.
+         * apply (eq_from_nth witness); first by rewrite !size_sub.
+           rewrite size_sub // => i?.
+           rewrite !nth_sub // get_setE // ifF 1:/# /=.
+           have ->: ltree_addr{1}.[i] = nth witness (sub ltree_addr{1} 0 3) i by rewrite nth_sub.
+           by rewrite H12 nth_sub.
+         * by rewrite -H23 to_uintK.
 
-seq 1 0 : (#pre /\ to_uint ots_addr{1}.[4] = s{2} + i{2}).
-    + inline {1}.
-      auto => /> &1 &2 ??????????????????<- *.
-      (* A seta refere se a hipotese sub ots_addr{1} 0 3 = sub address{2} 0 3 *)
-      apply (eq_from_nth witness); first by rewrite !size_sub.
-      rewrite size_sub // => j?.
-      by rewrite !nth_sub //= get_setE // ifF 1:/#.
+seq 1 4 : (
+  #{/~sub ots_addr{1} 0 5 = sub address{2} 0 5}
+   {/~ltree_addr{1}.[4] = (of_int (s{2} + i{2}))%W32}pre /\
+   val node{2} = to_list buf{1} /\ 
+   sub ots_addr{1} 0 3 = sub address{2} 0 3
+).
 
-(* ==================================================================================================================================================== *)
- 
-seq 1 6 : (#pre /\ to_list buf{1} = val node{2}).
-    + inline {1} M(Syscall).__gen_leaf_wots_ M(Syscall)._gen_leaf_wots M(Syscall).__gen_leaf_wots.
-      
-      seq 22 0 : (
-           #pre /\ 
-           ots_addr2{1} = ots_addr{1} /\
-           sk_seed2{1} = sk_seed{1} /\
-           pub_seed2{1} = pub_seed{1} /\
-           ltree_addr2{1} =  ltree_addr{1}
-      ); first by auto.
-          
-      seq 0 2 : (
-           #{/~ots_addr2{1} = ots_addr1{1}}
-            {/~sub ltree_addr{1} 0 3 = sub address{2} 0 3}pre /\ 
- 
-           sub ltree_addr{1} 0 3 = sub address{2} 0 3 /\
-           forall (k : int), 0 <= k < 5 => address{2}.[k] = ots_addr2{1}.[k]
+(* ===================================================================================================================== *)
+
+inline {1} M(Syscall).__gen_leaf_wots_ M(Syscall)._gen_leaf_wots M(Syscall).__gen_leaf_wots.             
+
+seq 22 0 : (
+    #pre /\
+  sk_seed2{1} = sk_seed{1} /\
+  pub_seed2{1} = pub_seed{1} /\
+  ots_addr2{1} = ots_addr{1} /\
+  ltree_addr2{1} = ltree_addr{1}
+); first by auto.
+
+seq 1 1 : (
+        #{/~ots_addr2{1} = ots_addr{1}}pre /\ 
+        pk{1} = DecodeWotsPk pk{2} /\
+        ots_addr2{1}.[0] = address{2}.[0] /\
+        ots_addr2{1}.[1] = address{2}.[1] /\
+        ots_addr2{1}.[2] = address{2}.[2] /\
+        ots_addr2{1}.[3] = W32.zero 
       ).
-         * auto => /> &1 &2 ???????????????H2?? H0 H3 ???? H1 *.
-           rewrite /set_type /set_ots_addr; do split.
-               - apply (eq_from_nth witness); first by rewrite !size_sub.
-                 rewrite size_sub // => j?.
-                 rewrite !nth_sub //= get_setE // ifF 1:/# get_setE //.
-                 case (j = 3) => //?.
-                 have ->: ots_addr{1}.[j] = nth witness (sub ots_addr{1} 0 3) j by rewrite nth_sub.
-                 by rewrite H0 nth_sub.
-               - apply (eq_from_nth witness); first by rewrite !size_sub.
-                 rewrite size_sub // => j?.
-                 rewrite !nth_sub //= get_setE // ifF 1:/# get_setE // ifF 1:/#.
-                 have ->: ltree_addr{1}.[j] = nth witness (sub ltree_addr{1} 0 3) j by rewrite nth_sub /#.
-                 rewrite H3 nth_sub // /#.
-               - move => k??.
-                 rewrite get_setE //.
-                 case (k = 4) => [-> |?].
-                      + by rewrite -H1 to_uintK.
-                 case (k = 3) => [-> |?]. 
-                      + by rewrite H2 get_setE.
-                 rewrite get_setE // ifF //.
-                 have ->: ots_addr{1}.[k] = nth witness (sub ots_addr{1} 0 3) k by rewrite nth_sub /#.
-                 rewrite H0 nth_sub /#.
+         * exists * sk_seed2{1}, pub_seed2{1}, ots_addr2{1}, address{2}.
+           elim * => P3 P4 P5 P6.
+           call {1} (pkgen_results P3 P4 P5 P6) => [/# |].
+           auto => /> &1 &2 H0 H1 H2 H3 H4 H5 H6 H7 H8 H9 H10 H11 H12 H13 H14 H15 H16 H17 H18 H19 H20 H21 H22 H23 H24 H25 *.
+           split => [| /#].
+           move => k*.
+           have ->: P5.[k] = nth witness (sub P5 0 5) k by rewrite nth_sub.
+           rewrite H24 nth_sub /#.
 
-      seq 1 1 : (
-          #{/~ots_addr2{1} = ots_addr{1}}
-           {/~forall (k : int), 0 <= k && k < 5 => address{2}.[k] = ots_addr2{1}.[k]}pre /\ 
-          pk{1} = DecodeWotsPk pk{2}
-      ). 
-         * exists * sk_seed2{1}, pub_seed2{1}; elim * => P0 P1.
-           call (pkgen_correct P0 P1) => [/#|].
-           skip => /> /#.
-      
-      seq 0 2 : (
-          #{/~sub ots_addr{1} 0 3 = sub address{2} 0 3}pre /\ 
-          forall (k : int), 0 <= k < 5 => ltree_addr2{1}.[k] = address{2}.[k]
+seq 0 2 : (
+          #{/~sub ots_addr{1} 0 5 = sub address{2} 0 5}pre /\ 
+          sub ltree_addr2{1} 0 5 = sub address{2} 0 5
       ).
+         * auto => /> &1 &2 H0 H1 H2 H3 H4 H5 H6 H7 H8 H9 H10 H11 H12 H13 H14 H15 H16 H17 H18 H19 H20 H21 H22 H23 H24 H25 H26 H27 H28 H29 *.
+           rewrite /set_ltree_addr /set_type.
+           do split; (
+              apply (eq_from_nth witness); [by rewrite !size_sub | rewrite size_sub // => i?];
+              rewrite !nth_sub // !get_setE //=
+           ).
+               - do (rewrite ifF 1:/#).
+                 have ->: ltree_addr{1}.[i] = nth witness (sub ltree_addr{1} 0 3) i by rewrite nth_sub.
+                 by rewrite H12 nth_sub.
+               - do (rewrite ifF 1:/#).
+                 have ->: node_addr{1}.[i] = nth witness (sub node_addr{1} 0 3) i by rewrite nth_sub.
+                 by rewrite H13 nth_sub.
+               - case (i = 4) => [-> /# |?].
+                 case (i = 3) => [-> /# |?].
+                 do (rewrite ifF 1:/#).
+                 have ->: ltree_addr{1}.[i] = nth witness (sub ltree_addr{1} 0 3) i by rewrite nth_sub /#.
+                 by rewrite H12 nth_sub /#.
 
-          * auto => /> &1 &2 ??????????????????????H1?H0 *; split => [| k??].
-               - apply (eq_from_nth witness); first by rewrite !size_sub.
-                 rewrite size_sub // => j?.
-                 by rewrite H0 !nth_sub //= /set_tree_addr /set_type get_setE // ifF 1:/# get_setE // ifF 1:/#.
-               - rewrite /set_ltree_addr /set_type get_setE //.
-                 case (k = 4) => [-> |?].
-                      + by rewrite -H1 to_uintK.
-                 rewrite get_setE //.
-                 case (k = 3) => //?.
-                 have ->: ltree_addr{1}.[k] = nth witness (sub ltree_addr{1} 0 3) k by rewrite nth_sub // /#.
-                 rewrite H0 nth_sub // /#.
+seq 1 1 : (
+          #{/~ltree_addr2{1} = ltree_addr{1}}pre /\ 
+          to_list leaf1{1} = val node{2} /\
+          ltree_addr2{1}.[0] = address{2}.[0] /\
+          ltree_addr2{1}.[1] = address{2}.[1] /\
+          ltree_addr2{1}.[2] = address{2}.[2] /\
+          ltree_addr2{1}.[3] = W32.one
+      ).
+         * exists * pk{1}, ltree_addr2{1}, pub_seed2{1}.
+           elim * => P0 P1 P2.
+           call (ltree_correct P0 P2 P1) => [/# |].
+           auto => /> &1 &2 *; split; [apply enc_dec_wots_pk => /# | smt(addr_sub_5)].
 
-      wp.
-      admit.
+auto => /> &1 &2 H0 H1 H2 H3 H4 H5 H6 H7 H8 H9 H10 H11 H12 H13 H14 H15 H16 H17 H18 H19 H20 H21 H22 H23 H24 H25 H26 H27 H28 H29 H30 H31 H32 H33 H34 *.
+      do split.
+         * apply (eq_from_nth witness); first by rewrite !size_sub.
+           rewrite size_sub // => i?. 
+           rewrite !nth_sub /#.
+         * by rewrite H30.
+         * apply (eq_from_nth witness); first by rewrite !size_sub.
+           rewrite size_sub // => i?. 
+           rewrite !nth_sub /#.
 
-(* ==================================================================================================================================================== *)
-
-seq 2 0 : (#pre /\ to_uint t64{1} = offset{2} * 32).
-          + auto => /> &1 &2 *.
-            rewrite to_uintM of_uintK //=/#.
-
-seq 1 1 : #pre.
-    + exists * _stack{1}, buf{1}, t64{1}; elim * => P0 P1 P2.
-      call {1} (memcpy_u8u8_3_352_32_post P0 P1 P2).
-      auto => /> &1 &2 H0 H1 H2 H3 H4 H5 H6 H7 H8 H9 H10 H11 H12 H13 H14 H15 H16 H17 H18 H19 H20 H21 H22 H23 H24 H25 H26 *; do split.
-          - rewrite H26 /#.
-          - rewrite h_val d_val /= in H7.
-            move: H6; rewrite H7 => H6.
-            rewrite H26.  admit. (* Isto e falso *)
-          - move => ?? r H; do split.
-              * rewrite size_put /#.
-              * rewrite size_put /#.
-              * apply (eq_from_nth witness); first by rewrite size_sub 1:/# size_sub_list // /#.
-                rewrite size_sub 1:/# n_val => j?.
-                rewrite nth_sub 1:/# /= /sub_list nth_mkseq //= /nbytes_flatten (nth_flatten witness n).
-                     + admit.
-                rewrite (nth_map witness).
-                     + rewrite size_put /#.
-                rewrite nth_put 1:/# ifF 1:/#.
-                admit.
-
-
-seq 2 2 : #{/~to_uint t64{1} = offset{2} * 32}pre.
-          + auto => /> &1 &2 H0 H1 H2 H3 H4 H5 H6 H7 H8 H9 H10 H11 H12 H13 H14 H15 H16 H17 H18 H19 H20 H21 H22 H23 H24 H25 H26; do split.
-               * rewrite to_uintD /#.
-               * smt().
-               * smt().
-               * rewrite H7 d_val h_val /=. admit.
-               * by rewrite size_put H8.
-               * apply (eq_from_nth witness); first by rewrite size_sub_list 1:/# size_map size_sub 1:/#.
-                 rewrite size_map size_sub 1:/# => j?.
-                 rewrite /sub_list nth_mkseq //= (nth_map witness).
-                     + rewrite size_sub /#.
-                 rewrite nth_sub // nth_put.
-                     + admit.
-                 case (to_uint offset{1} = j) => H.
-                     + rewrite get_setE /=.
-                         * admit. 
-                       rewrite ifT //. 
-                       smt(@W64 pow2_64).
-                     + rewrite get_setE /=.
-                         * admit.
-                       rewrite ifF 1:#smt:(@W64 pow2_64).
-                       have ->: nth witness heights{2} j = nth witness (sub_list heights{2} 0 (to_uint offset{1})) j by rewrite /sub_list nth_mkseq 1:/#.
-                       rewrite -H13 (nth_map witness).
-                         * rewrite size_sub //#.
-                       by rewrite nth_sub 1:/#.
-               
-               * apply (eq_from_nth witness); first by rewrite size_sub 1:/# size_sub_list /#.
-                 rewrite size_sub 1:/# n_val => j?.
-                 rewrite nth_sub 1:/# /sub_list nth_mkseq //= /nbytes_flatten (nth_flatten witness n).
-                         * pose P := (fun (s0 : W8.t list) => size s0 = n).
-                           pose L := (map NBytes.val stack{2}).
-                           rewrite -(all_nthP P L witness) /P /L size_map H7 d_val h_val /= => k?. 
-                           by rewrite (nth_map witness) 1:/# valP. 
-                 rewrite (nth_map witness).
-                         * admit.
-                 admit.
+(* ===================================================================================================================== *)
+  
+seq 2 0 : (#pre /\ to_uint t64{1} = offset{2} * 32); first by auto => /> *; rewrite to_uintM of_uintK /=/#.
+ 
+seq 3 3 : ( 
+  #{/~to_uint t64{1} = offset{2} * 32}{/~0 <= offset{2}}{/~offset{2} < size heights{2}}pre /\
+   0 < offset{2} <= size heights{2}
+).
+    + wp. 
+      exists * _stack{1}, buf{1}, t64{1}; elim * => P3 P4 P5.
+      call {1} (memcpy_u8u8_3_352_32_post P3 P4 P5).
+      auto => /> &1 &2 H0 H1 H2 H3 H4 H5 H6 H7 H8 H9 H10 H11 H12 H13 H14 H15 H16 H17 H18 H19 H20 H21 H22 H23 H24 H25 -> *.
+      do split; 1,2: by smt(). 
+      move => H26 H27 result H29 H30 H31 *.
+      rewrite !size_put.  
+      do split; 2..4,8,9: by smt(). 
+            + rewrite to_uintD /#.  
+            + apply (eq_from_nth witness); first by rewrite size_map size_sub 1:/# size_sub_list ///#.
+           rewrite size_map size_sub 1:/# => j?.
+           rewrite /sub_list nth_mkseq //= nth_put 1:/#.
+           rewrite (nth_map witness); first by rewrite size_sub /#.
+           rewrite nth_sub // get_setE // to_uintB /=; 1,3: by rewrite uleE to_uintD /#.
+              - rewrite to_uintD /#.
+           case (j = to_uint offset{1}) => [-> |?].
+              - by rewrite ifT //= to_uintD /#.
+              - rewrite ifF /=; first by rewrite to_uintD /#.     
+                rewrite ifF 1:/#.
+                have ->:  nth witness heights{2} j = nth witness (sub_list heights{2} 0 (to_uint offset{1})) j by rewrite /sub_list nth_mkseq 1:/#.
+                rewrite -H18 (nth_map witness); first by rewrite size_sub /#.
+                by rewrite nth_sub /#.
+            + by move => *; rewrite !nth_put /#.
+            + rewrite n_val; apply (eq_from_nth witness); first by rewrite size_sub 1:/# size_sub_list /#.
+              rewrite size_sub 1:/# => j?.
+              rewrite nth_sub 1:/# /= /sub_list nth_mkseq 1:/# /= nth_nbytes_flatten; first by rewrite size_put /#.
+              rewrite nth_put 1:/#.
+              case (to_uint offset{1} = j %/ n) => H.
+                  * rewrite H24 get_to_list /= -H30 /#.
+                  * have ->: nth witness (val (nth witness stack{2} (j %/ n))) (j %% n) = nth witness (sub_list (nbytes_flatten stack{2}) 0 (n * to_uint offset{1})) j by rewrite /sub_list nth_mkseq 1:/# /= nth_nbytes_flatten // /#.
+                    rewrite -H20 nth_sub 1:/# /= /#. 
 
 seq 1 0 : (
     #pre /\ 
-    if treehash_cond heights{1} offset{1} then cond{1} = W8.one else cond{1} = W8.zero
+    (cond{1} = W8.one) = (2 <= offset{2} /\ heights{1}.[to_uint offset{1} - 2] = heights{1}.[to_uint offset{1} - 1])
 ).
-    + ecall {1} (treehash_cond_correct_p heights{1} offset{1}).
-      auto => /> /#.
+    + ecall {1} (p_treehash_condition_correct_eq heights{1} offset{1}).
+      auto => /> &1 &2 /#.
 
-while (#pre); first by admit.
-    + skip => /> &1 &2 H0 H1 H2 H3 H4 H5 H6 H7 H8 H9 H10 H11 H12 H13 H14 H15 H16 H17 H18 H19 H20 H21 H22 H23 H24 H25 H26 *; do split.
-         * move => H27.
-           have E: treehash_cond heights{1} offset{1}.
-              move: H26.
-              move: H27. 
-           admit.
-         * admit. (* Treehash cond needs to be an smequivalence *)
-         * move => ?. 
-           have ->: nth witness heights{2} (to_uint offset{1} - 1) = nth witness (sub_list heights{2} 0 (to_uint offset{1})) (to_uint offset{1} - 1) by rewrite /sub_list nth_mkseq /#.
-           have ->: nth witness heights{2} (to_uint offset{1} - 2) = nth witness (sub_list heights{2} 0 (to_uint offset{1})) (to_uint offset{1} - 2) by rewrite /sub_list nth_mkseq /#.
-           rewrite -H13 !(nth_map witness) //=. 
-              + rewrite size_sub /#.
-              + rewrite size_iota /#.
-              + rewrite size_sub /#.
-              + rewrite size_iota /#.
-           rewrite nth_iota 1:/# nth_iota 1:/# /= => H30.
-           have := H26.
-           rewrite /treehash_cond ifT; split => [/# |].
-           smt(@W32 pow2_32).
-         * move => stackImpl bufL heightsImpl node_addr offsetImpl addrSpec heighrsSpec stackSpec.
-         * move => H31 H32 H33 H34 H35 H36 H37 H38 H39 H40 H41 H42 H43 H44*; do split.
-               - admit.
-               - smt().
-               - smt().
-               - admit.
-               - smt(@W32 pow2_32).
-               - rewrite ultE; smt(@W32 pow2_32).
-               - rewrite ultE; smt(@W32 pow2_32).
-qed.
+seq 0 1 : (#pre /\ sub node_addr{1} 0 5 = sub address{2} 0 5).
+    + auto => /> &1 &2 H0 H1 H2 H3 H4 H5 H6 H7 H8 H9 H10 H11 H12 H13 H14 H15 H16 H17 H18 H19 H20 H21 H22 H23 H24 H25 H26.
+      rewrite /set_type.
+      do split; (apply (eq_from_nth witness); [by rewrite !size_sub| rewrite size_sub // => i?]; rewrite !nth_sub //= !get_setE //).
+         - do (rewrite ifF 1:/#).
+           have ->: ltree_addr{1}.[i] = nth witness (sub ltree_addr{1} 0 3) i by rewrite nth_sub.
+           by rewrite H10 nth_sub.
+         - do (rewrite ifF 1:/#).
+           have ->: node_addr{1}.[i] = nth witness (sub node_addr{1} 0 3) i by rewrite nth_sub.
+           by rewrite H11 nth_sub.
+         - do (rewrite ifF 1:/#).
+           have ->: ots_addr{1}.[i] = nth witness (sub ots_addr{1} 0 3) i by rewrite nth_sub.
+           by rewrite H23 nth_sub.
+         - case (i = 3) => //?. 
+           case (i = 4) => //?.
+           do (rewrite ifF 1:/#).
+           have ->: node_addr{1}.[i] = nth witness (sub node_addr{1} 0 3) i by rewrite nth_sub /#.
+           by rewrite H11 nth_sub /#.
 
-lemma build_auth_path_correct (_pub_seed _sk_seed : W8.t Array32.t, _idx : W32.t, a : adrs) :
-    len = XMSS_WOTS_LEN /\ 
-    n = XMSS_N /\
-    d = XMSS_D /\
-    h = XMSS_TREE_HEIGHT =>
-    equiv[
-      M(Syscall).__build_auth_path ~ TreeSig.buildAuthPath :
-      arg{1}.`2 = _sk_seed /\
-      arg{1}.`3 = _pub_seed /\
-      arg{1}.`4 = _idx /\
-      arg{1}.`5 = a /\
+conseq /> => [/# |]. (* simplifies #post *)
 
-      arg{2}.`1 = NBytes.insubd (to_list _pub_seed) /\
-      arg{2}.`2 = NBytes.insubd (to_list _sk_seed) /\
-      arg{2}.`3 = _idx /\
-      arg{2}.`4 = a /\
-
-      0 <= to_uint _idx < 2 ^ XMSS_FULL_HEIGHT - 1
-      ==>
-      res{2} = EncodeAuthPath (to_list res{1})
-    ].
-proof.
-rewrite /XMSS_WOTS_LEN /XMSS_N /XMSS_D /XMSS_TREE_HEIGHT => [#] len_val n_val d_val h_val.
-proc => /=.
-seq 2 3 : (#pre /\ ={j} /\ j{1} = 0 /\ size authentication_path{2} = h). 
-  + auto => />; by rewrite size_nseq h_val.
-
-(* With this conseq, proving the last subgoal of the while loop becomes much easier *)
-conseq (: _ ==> 
-  to_list auth_path{1} = nbytes_flatten authentication_path{2} /\
-  size authentication_path{2} = h
-).
-  + auto => /> &1 &2 H0 H1 l r -> H.
-    (* A seta refere se a hipotese to_list `auth_path_L = nbytes_flatten `authentication_path_R *)
-    apply auth_path_eq.
-    rewrite /EncodeAuthPath /nbytes_flatten !insubdK.
-        * by rewrite /P.
-        * rewrite /P size_map size_chunk 1:/# size_nbytes_flatten /#.
-    apply (eq_from_nth witness).
-        * rewrite size_map size_chunk 1:/# size_nbytes_flatten /#.
-    rewrite H h_val => i?.
-    rewrite (nth_map witness). 
-        * rewrite size_chunk 1:/# size_nbytes_flatten /#.
-    rewrite /chunk nth_mkseq.
-        * rewrite size_nbytes_flatten /#.
-    apply nbytes_eq; apply (eq_from_nth witness); first by rewrite !valP.
-    rewrite valP n_val => j?.
-    rewrite insubdK => />.
-        * rewrite /P size_take 1:/# size_drop 1:/# size_nbytes_flatten /#.
-    rewrite nth_take 1,2:/# nth_drop 1,2:/# (nth_flatten witness n).
-        * pose P := (fun (s : W8.t list) => size s = n).
-          pose L := (map NBytes.val r).
-          rewrite -(all_nthP P L witness) /P /L size_map H h_val => k?.
-          by rewrite (nth_map witness) 1:/# valP.
-    rewrite (nth_map witness) /#.
-
-(* Rewrite #pre *)
-conseq ( :
-  to_list sk_seed{1} = val sk_seed{2} /\
-  to_list pub_seed{1} = val pub_seed{2} /\
-  addr{1} = address{2} /\
-  ={j} /\ j{1} = 0 /\
-  i{1} = idx{2} /\ 
-  0 <= to_uint idx{2} < 2 ^ XMSS_FULL_HEIGHT - 1 /\
-  size authentication_path{2} = 10
-  ==> _
-).
-    + auto => /> *; split.
-        * apply (eq_from_nth witness); first by rewrite valP size_to_list n_val.
-          rewrite size_to_list => j?.
-          by rewrite insubdK // /P size_to_list n_val.
-        * split => [| /#].
-          apply (eq_from_nth witness); first by rewrite valP size_to_list n_val.
-          rewrite size_to_list => j?.
-          by rewrite insubdK // /P size_to_list n_val.
-
-while (
-  to_list sk_seed{1} = val sk_seed{2} /\
-  to_list pub_seed{1} = val pub_seed{2} /\
-  addr{1} = address{2} /\
-  i{1} = idx{2} /\
-  ={j} /\ 0 <= j{2} <= 10 /\ 
-  size authentication_path{2} = 10 /\
-
-  (0 <= to_uint idx{2} < 2 ^ XMSS_FULL_HEIGHT - 1) /\
-
-  forall (k : int), 0 <= k < n * j{1} => auth_path{1}.[k] = nth witness (nbytes_flatten authentication_path{2}) k
-); last first.
-    + auto => /> &1 &2 ?????.
-      split => [/# | authL authR j ????H0].
-      have ->: j = h by smt().
-      rewrite n_val h_val /= => H1.
-      split => [| /#].
-      apply (eq_from_nth witness); first by rewrite size_to_list size_nbytes_flatten_2 H0 n_val.
-      rewrite size_to_list => ??.
-      by rewrite  get_to_list H1.
-
- 
-seq 4 1 : (
-    #pre /\ 
-    to_uint k{1} = k{2} * 2^j{1} /\
-    k{2} = to_uint ((idx{2} `>>` (of_int j{2})%W8) `^` W32.one)
-).
-    + auto => /> &1 &2 ? H *.
-      rewrite /XMSS_FULL_HEIGHT /= in H.
-      rewrite shl_shlw 1:/# /(`>>`) of_uintK to_uint_shl //. 
-      admit.
-
-seq 1 1 : (#pre /\ to_list node{1} = val t{2}).
-    + inline {1} 1.
-      inline {1} 13.
-      wp; sp.
-      exists * pub_seed{1}, sk_seed{1}, k{1}, (of_int j{1})%W32, addr{1}.
-      elim * => P0 P1 P2 P3 P4.
-      call {1} (treehash_correct P1 P0 P2 P3 P4) => [/# |].
-      skip => /> &1 &2 H0 H1 H2 H3 H4 H5 H6 H7 H8 H9 ->.
-      do split; 1,2:smt(@NBytes).
-         * rewrite of_uintK /#.
-         * rewrite of_uintK /#.
-         * smt(@W32 pow2_32).
-         * admit.
-         * rewrite of_uintK => *.
-           admit.            
-
-
-auto => /> &1 &2 H0 H1 H2 H3 H4 H5 H6 H7 H8 H9 H10 H11; do split; 1,2,5,6: by smt().
-    - by rewrite size_put.
-    - move => k??.
-
-rewrite initiE 1:/# /= /nbytes_flatten (nth_flatten witness 32).
-    + pose P := (fun (s : W8.t list) => size s = 32).
-      pose L := (map NBytes.val (put authentication_path{2} j{2} t{2})).
-      rewrite -(all_nthP P L witness) /P /L size_map size_put H4 => i?.
-      rewrite (nth_map witness); first by rewrite size_put /#.
-      by rewrite valP n_val.
-
-rewrite (nth_map witness); first by rewrite size_put /#.
-rewrite nth_put 1:/#.
-
-case (j{2} * 32 <= k && k < j{2} * 32 + 32) => ?.
-    + rewrite ifT 1:/# -H11 get_to_list /#.
-    + rewrite ifF 1:/# H7 1:/# /nbytes_flatten (nth_flatten witness 32).
-         - pose P := (fun (s : W8.t list) => size s = 32).
-           pose L := (map NBytes.val authentication_path{2}).
-           rewrite -(all_nthP P L witness) /P /L size_map => ??.
-           by rewrite (nth_map witness) 1:/# valP n_val.
-      by rewrite (nth_map witness) 1:/#.
-qed.
-
-
-lemma treesig_correct (_m : W8.t Array32.t, _sk : xmss_sk, _idx_sig : W32.t, _addr : W32.t Array8.t) :
-    n = XMSS_N /\
-    len = XMSS_WOTS_LEN /\ 
-    d = XMSS_D /\
-    h = XMSS_TREE_HEIGHT /\ 
-    floor (log2 w%r) = XMSS_WOTS_LOG_W /\ 
-    w = XMSS_WOTS_W /\ 
-    len1 = XMSS_WOTS_LEN1 /\ 
-    len2 = XMSS_WOTS_LEN2
- =>
-    equiv [
-      M(Syscall).__tree_sig ~ TreeSig.treesig:
-      arg{1}.`2 = _m /\
-      arg{1}.`3 = DecodeSkNoOID _sk /\
-      arg{1}.`4 = _idx_sig /\
-      arg{1}.`5 = _addr /\
       
-      arg{2}.`1 = NBytes.insubd (to_list _m) /\
-      arg{2}.`2 = _sk /\
-      arg{2}.`3 = _idx_sig /\
-      arg{2}.`4 = _addr /\
+while (
+  t{2} = to_uint target_height{1} /\
+  0 <= t{2} <= h /\
 
-      (* Isto e a negacao da condicao idx >= ((1ULL << params->full_height) - 1) usada p verificar se ainda se pode assinat com uma determinada chave *)
-      (* FIXME: e 2^XMSS_FULL_HEIGHT - 1 e nao 2^XMSS_FULL_HEIGHT *)
-      0 <= to_uint _idx_sig < 2 ^ XMSS_FULL_HEIGHT - 1
+  s{2} = to_uint start_index{1} /\
+  0 <= s{2} <= h /\
 
-      ==>
-      res{2} = EncodeReducedSignature (to_list res{1}.`1)
-    ].
-proof.
-rewrite /XMSS_N /XMSS_WOTS_LEN /XMSS_D /XMSS_TREE_HEIGHT /XMSS_WOTS_LOG_W.
-rewrite /XMSS_WOTS_W /XMSS_WOTS_LEN1 /XMSS_WOTS_LEN2.
-move => [#] n_val len_val d_val h_val logw_val w_val len1_val len2_val.
-proc => /=.
-seq 6 0 : (
-  #pre /\
-  to_list pub_seed{1} = sub sk{1} (XMSS_INDEX_BYTES + 3*32) 32 /\
-  to_list sk_seed{1} = sub sk{1} XMSS_INDEX_BYTES 32
-).
-    + auto => /> *; split.
-         * apply (eq_from_nth witness); first by rewrite size_to_list size_sub.
-           rewrite size_to_list => i?.
-           rewrite get_to_list initiE // nth_sub //.
-         * apply (eq_from_nth witness); first by rewrite size_to_list size_sub.
-           rewrite size_to_list => i?.
-           by rewrite get_to_list initiE // nth_sub.
+  offset{2} = to_uint offset{1} /\
+  (i{2} <> 0 => 0 < offset{2}) /\
+  0 <= i{2} <= 2 ^ t{2} /\
+  to_uint i{1} = i{2} /\
+  to_uint upper_bound{1} = 2 ^ t{2} /\
 
-seq 0 2 : (
-  #pre /\
-  val sk_seed{2} = to_list sk_seed{1} /\
-  val pub_seed{2} = to_list pub_seed{1}
-).
-    + auto => /> &1 ?? -> ->; split; rewrite /DecodeSkNoOID.
-       * apply (eq_from_nth witness); first by rewrite valP size_sub.
-         rewrite valP n_val => i?.
-         rewrite nth_sub // get_of_list 1:/#.
-         rewrite nth_cat ifT.
-             - rewrite !size_cat valP n_val size_take //.
-               rewrite ifT; [by rewrite size_W32toBytes |].
-               rewrite !valP /#.
-         rewrite nth_cat ifT.
-             - rewrite !size_cat valP n_val size_take //.
-               rewrite ifT; [by rewrite size_W32toBytes |].
-               rewrite !valP /#.
-         rewrite nth_cat ifT.
-             - rewrite !size_cat valP n_val size_take //.
-               rewrite ifT; [by rewrite size_W32toBytes | smt()].
-         rewrite nth_cat ifF; [by rewrite size_take // size_W32toBytes /# |].
-         rewrite size_take // size_W32toBytes /#.
-       * apply (eq_from_nth witness); first by rewrite valP n_val size_sub.
-         rewrite valP n_val => i?.
-         rewrite nth_sub // get_of_list 1:/# nth_cat ifF.
-             - rewrite !size_cat !valP n_val size_take // size_W32toBytes /#.
-         rewrite !size_cat !valP n_val size_take // size_W32toBytes /#.
+  size stack{2} = h %/ d + 1 /\
+  size heights{2} = h %/ d + 1 /\
 
-(* Rewrite #pre *)
-conseq (:
-  M{2} = (insubd (to_list m{1}))%NBytes /\
-  idx{2} = idx_sig{1} /\
-  address{2} = addr{1} /\
-  val sk_seed{2} = to_list sk_seed{1} /\
-  val pub_seed{2} = to_list pub_seed{1} /\
-  0 <= to_uint idx_sig{1} < 2 ^ XMSS_FULL_HEIGHT - 1
-  ==>
-  _
-); first by auto.
+  sk_seed{2} = (insubd (to_list sk_seed{1}))%NBytes /\
+  pub_seed{2} = (insubd (to_list pub_seed{1}))%NBytes /\
+
+  sub ltree_addr{1} 0 3 = sub address{2} 0 3 /\
+  sub node_addr{1} 0 5 = sub address{2} 0 5 /\
+  sub ots_addr{1} 0 3 = sub address{2} 0 3 /\
+  
+  ots_addr{1}.[3] = W32.zero /\
+  ltree_addr{1}.[3] = W32.one /\
+  node_addr{1}.[3] = (of_int 2)%W32 /\
+  node_addr{1}.[4] = W32.zero /\
+
+  map W32.to_uint (sub heights{1} 0 offset{2}) = sub_list heights{2} 0 offset{2} /\
+
+  (forall (k : int), 0 <= k < offset{2} => 0 <= nth witness heights{2} k < XMSS_TREE_HEIGHT) /\
+
+  sub _stack{1} 0 (n * offset{2}) = sub_list (nbytes_flatten stack{2}) 0 (n * offset{2}) /\
+
+  i{2} < 2 ^ t{2} /\
+
+  (cond{1} = W8.one) = (2 <= offset{2} /\ heights{1}.[to_uint offset{1} - 2] = heights{1}.[to_uint offset{1} - 1]) /\
+  
+  0 < offset{2} <= size heights{2} 
+(*  ((heights{1}.[to_uint offset{1} - 2] = heights{1}.[to_uint offset{1} - 1]) => (offset{2} < size heights{2})) *)
+(* This is not true before the loop starts *)
+); last first. 
+
+    + auto => /> &1 &2 H0 H1 H2 H3 H4 H5 H6 H7 H8 H9 H10 H11 H12 H13 H14 H15 H16 H17 H18 H19 H20 H21 H22 H23 H24 H25 -> H27 *.
+      do split.  
+        * move => [Ha Hb].
+          split; first by assumption.
+          have ->: nth witness heights{2} (to_uint offset{1} - 2) = nth witness (sub_list heights{2} 0 (to_uint offset{1})) (to_uint offset{1} - 2) by rewrite /sub_list nth_mkseq /#.
+          have ->: nth witness heights{2} (to_uint offset{1} - 1) = nth witness (sub_list heights{2} 0 (to_uint offset{1})) (to_uint offset{1} - 1) by rewrite /sub_list nth_mkseq /#. 
+          rewrite -H16.
+          rewrite (nth_map witness); first by rewrite size_sub /#.
+          rewrite nth_sub 1:/# /= -Hb.
+          rewrite (nth_map witness); first by rewrite size_sub /#.
+          by rewrite nth_sub 1:/#.
+        * move => ?.
+          have ->: nth witness heights{2} (to_uint offset{1} - 2) = nth witness (sub_list heights{2} 0 (to_uint offset{1})) (to_uint offset{1} - 2) by rewrite /sub_list nth_mkseq /#.
+          have ->: nth witness heights{2} (to_uint offset{1} - 1) = nth witness (sub_list heights{2} 0 (to_uint offset{1})) (to_uint offset{1} - 1) by rewrite /sub_list nth_mkseq /#.
+          rewrite -H16.
+          rewrite (nth_map witness); first by rewrite size_sub /#.
+          rewrite  nth_sub 1:/# /=.
+          rewrite (nth_map witness); first by rewrite size_sub /#.
+          rewrite  nth_sub 1:/# /= => ?.
+          smt(@W32 pow2_32).
  
-seq 1 1 : (#pre /\ auth{2} = EncodeAuthPath (to_list auth_path{1})).
-    + exists * pub_seed{1}, sk_seed{1}, idx_sig{1}, addr{1}.
-      elim * => P0 P1 P2 P3.
-      call (build_auth_path_correct P0 P1 P2 P3) => [/# |].
-      skip => /> &2 <- <- ??; by smt(@NBytes).
+        * move => _stack_L cond_L heights_L node_addr_L offset_L address_R heights_R stack_R.
+          move => H28 H29 H30 H31 H32 H33 H34 H35 H36 H37 H38 H39 H40 H41 H42 H43.
+          have E1 : 2 ^ to_uint target_height{1} <= 2^h by smt(@RealExp).
+          have E2 : to_uint i{1} <= 2^h by smt(@RealExp).
+          rewrite E0 in E2.
+          do split.
+            * smt(). 
+            * move => ?. rewrite H32 h_val d_val /=. 
+              have E29: (to_uint offset_L <= 2) \/ (nth witness heights_R (to_uint offset_L - 1) <> nth witness heights_R (to_uint offset_L - 2)) by smt().
+              have := E29.
+              move => [? /# | ?].
+              rewrite H32 h_val d_val /= in H43.
+             admit. (* 0 <= to_uint offset_L => to_uint offset_L < size heights_R *)
+            * smt().
+            * smt().
+            * rewrite to_uintD /#.
+            * smt(sub_N).
+            * smt().
+            * rewrite ultE to_uintD /#.
+            * rewrite ultE to_uintD /#.
 
-seq 2 2 : (#pre); first by inline {1}; auto.
+seq 2 0 : (#pre /\ to_uint tree_idx{1} = s{2} + i{2}).
+    + auto => /> &1 *. 
+      have ?: 0 <= 2 ^ to_uint target_height{1} <= 1048576 by smt(@RealExp).
+      rewrite to_uintD_small // /#.
 
-seq 1 1 : (sig_ots{2} = EncodeWotsSignature sig_ots{1} /\ auth{2} = EncodeAuthPath (to_list auth_path{1})).
-    + inline {1} M(Syscall).__wots_sign_ M(Syscall)._wots_sign.
-      sp; wp.
-      exists * msg0{1}, seed0{1}, pub_seed{1}, addr1{1}.
-      elim * => P0 P1 P2 P3.
-      call {1} (wots_sign_seed_corect P0 P1 P2 P3) => [/# |]. 
-      skip => /> &1 &2 <- <- *; do split.
-           - by rewrite insubdK /P // size_to_list n_val.
-           - smt(@NBytes).
-           - smt(@NBytes).
+seq 2 0 : (#pre /\ to_uint u{1} = nth witness heights{2} (offset{2} - 1) + 1).
+    + auto => /> &1 &2 H0 H1 H2 H3 H4 H5 H6 H7 H8 H9 H10 H11 H12 H13 H14 H15 H16 H17 H18 H19 H20 H21 H22 H23 H24 H25 H26.
+      have ->: nth witness heights{2} (to_uint offset{1} - 1) = nth witness (sub_list heights{2} 0 (to_uint offset{1})) (to_uint offset{1} - 1) by rewrite /sub_list nth_mkseq /#.
+      rewrite -H17.
+      rewrite (nth_map witness); first by rewrite size_sub /#.
+      rewrite nth_sub 1:/# /=.
+      have ->: to_uint (offset{1} - W64.one) = to_uint offset{1} - 1 by rewrite to_uintB // uleE /#.
+      rewrite to_uintD_small //=.
+      have ->: to_uint heights{1}.[to_uint offset{1} - 1] = nth witness (map W32.to_uint (sub heights{1} 0 (to_uint offset{1}))) (to_uint offset{1} - 1).
+          *  rewrite (nth_map witness); [by rewrite size_sub /# | by rewrite nth_sub /#]. 
+      rewrite H17 (nth_map witness); first by rewrite size_iota /#.
+      rewrite /= nth_iota 1:/# /=.
+      smt(@W32 pow2_32).
 
-seq 2 0 : (#pre /\ sub sig{1} 0 XMSS_WOTS_SIG_BYTES = to_list sig_ots{1}).
-    + while {1} 
-      (#pre /\ 
-       0 <= i{1} <= 2144 /\
-       forall (k : int), 0 <= k < i{1} => sig{1}.[k] = sig_ots{1}.[k])
-      (2144 - i{1}); last first.
-           * auto => /> &1; split => [/# | i sig].
-             split => [/# | ???].
-             have ->: i = 2144 by smt().
-             move => H. 
-             apply (eq_from_nth witness); first by rewrite size_to_list size_sub.
-             rewrite size_sub // => j?.
-             rewrite nth_sub //=. 
-             by apply H.
-      auto => /> &hr ?? H*; do split; 1,2,4: by smt().
-      move => k??.
-      rewrite get_setE 1:/#.
-      case (k = i{hr}) => [-> // | ?].
-      apply H => /#.
- 
-seq 3 0 : (#pre /\ sub sig{1} XMSS_WOTS_SIG_BYTES 320 = to_list auth_path{1}).
-    + while {1} 
-      (#pre /\ 
-       aux{1} = 320 /\
-       0 <= i{1} <= 320 /\
-       forall (k : int), 0 <= k < i{1} => sig{1}.[XMSS_WOTS_SIG_BYTES + k] = auth_path{1}.[k])
-      (320 - i{1}); last first.
-           * auto => /> &1 ?; split => [/# | i sig].
-             split => [/# | ????].
-             have ->: i = 320 by smt().
-             move => H. 
-             apply (eq_from_nth witness); first by rewrite size_to_list size_sub.
-             rewrite size_sub // => j?.
-             rewrite nth_sub //=. 
-             by apply H.
-      auto => /> &hr H *; do split; 2,3,5: by smt().
-           * apply (eq_from_nth witness); first by rewrite size_to_list size_sub.
-             rewrite size_sub // /XMSS_WOTS_SIG_BYTES => j?.
-             by rewrite nth_sub // -H get_setE 1:/# ifF 1:/# /= nth_sub.
-           * move => k??.
-             rewrite get_setE 1:/#.
-             case (k = i{hr}) => [-> // | ?].
-             rewrite ifF /#.
+seq 1 1 : (#{/~to_uint tree_idx{1} = s{2} + i{2}}pre /\ tree_idx{1} = tree_index{2}).
+    + auto => /> &1 &2 H0 H1 H2 H3 H4 H5 H6 H7 H8 H9 H10 H11 H12 H13 H14 H15 H16 H17 H18 H19 H20 H21 H22 H23 H24 H25 H26 H27.
+      rewrite (: 31 = 2^5 - 1) 1:/# and_mod //.
+      rewrite /(`>>`) to_uint_truncateu8 of_uintK modz_small #smt:(@W32 @W8 @IntDiv). 
 
-auto => /> &1 H0 H1.
-rewrite /EncodeReducedSignature.
-rewrite /XMSS_WOTS_SIG_BYTES in H0.
-rewrite /XMSS_WOTS_SIG_BYTES in H1.
-congr.
-        + rewrite encodewotssig_list_array; congr.
-          rewrite -H0.
-          apply (eq_from_nth witness); first by rewrite size_sub // size_sub_list.
+seq 2 2 : (
+    #{/~sub node_addr{1} 0 3 = sub address{2} 0 3}{~sub node_addr{1} 0 4 = sub address{2} 0 4}pre /\ 
+    sub node_addr{1} 0 7 = sub address{2} 0 7
+).
+    + inline {1}.
+      auto => /> &1 &2 H0 H1 H2 H3 H4 H5 H6 H7 H8 H9 H10 H11 H12 H13 H14 H15 H16 H17 H18 H19 H20 H21 H22 H23 H24 H25 H26*.
+      rewrite /set_tree_index /set_tree_height.
+      do split; (
+         apply (eq_from_nth witness); [by rewrite !size_sub | rewrite size_sub // => i?]; 
+         rewrite !nth_sub // !get_setE //=
+      ); 1..3:smt(sub_k sub_N).
+         - case (i = 6) => //?.
+           case (i = 5) => //?.
+             + have ->: heights{1}.[to_uint (offset{1} - W64.one)] = W32.of_int (nth witness (map W32.to_uint (sub heights{1} 0 (to_uint offset{1}))) (to_uint offset{1} - 1)).
+                   - rewrite (nth_map witness); first by rewrite size_sub /#. 
+                     rewrite nth_sub 1:/# /=. 
+                     congr.
+                     by rewrite to_uintB // uleE /#.    
+               congr; rewrite H17 /sub_list nth_mkseq /#. 
+           have ->: node_addr{1}.[i] = nth witness (sub node_addr{1} 0 5) i by rewrite nth_sub /#.                    
+           rewrite H11 nth_sub /#.              
+
+conseq /> => [/# |].
+
+seq 4 2 : (#pre /\ to_list buf2{1} = val node0{2} ++ val node1{2}).
+        + ecall {1} (memcpy_u8u8_2_64_352_post buf2{1} _stack{1} t64{1}).
+          auto => /> &1 &2 H0 H1 H2 H3 H4 H5 H6 H7 H8 H9 H10 H11 H12 H13 H14 H15 H16 H17 H18 H19 H20 H21 H22 H23 H24 H25 H26 H27 result ->.
+          apply (eq_from_nth witness); first by rewrite size_sub // size_cat !valP n_val.
           rewrite size_sub // => j?.
-          by rewrite nth_sub // /sub_list nth_mkseq .
-        + congr.
-          apply (eq_from_nth witness); first by rewrite size_to_list size_sub_list.
-          rewrite size_to_list => j?.
-          by rewrite -H1 nth_sub // /sub_list nth_mkseq.
-qed.
+          case (0 <= j < 32) => ?; last first.
+             - rewrite nth_sub // nth_cat valP ifF 1:/#.
+               have ->: to_uint ((offset{1} - (of_int 2)%W64) * (of_int 32)%W64) + j = (to_uint offset{1} - 2) * 32 + j.
+                   + rewrite to_uintM of_uintK /= to_uintB; first by rewrite uleE /#.
+                     rewrite of_uintK /#.
+               have ->: _stack{1}.[(to_uint offset{1} - 2) * 32 + j] = nth witness (sub _stack{1} 0 (n * to_uint offset{1})) ((to_uint offset{1} - 2) * 32 + j) by rewrite nth_sub /#.
+               rewrite H19.
+               rewrite /sub_list nth_mkseq 1:/# /= nth_nbytes_flatten /#.
+             - rewrite nth_sub // nth_cat valP ifT 1:/#.
+               have ->: to_uint ((offset{1} - (of_int 2)%W64) * (of_int 32)%W64) + j = (to_uint offset{1} - 2) * 32 + j.
+                   + rewrite to_uintM of_uintK /= to_uintB; first by rewrite uleE /#.
+                     rewrite of_uintK /#.
+               have ->: _stack{1}.[(to_uint offset{1} - 2) * 32 + j] = nth witness (sub _stack{1} 0 (n * to_uint offset{1})) ((to_uint offset{1} - 2) * 32 + j) by rewrite nth_sub /#.
+               rewrite H19.
+               rewrite /sub_list nth_mkseq 1:/# /= nth_nbytes_flatten /#.
+ 
+seq 1 1 : (#{/~val node{2} = to_list buf{1}}pre /\ to_list buf{1} = val new_node{2}).
+          + inline {1} M(Syscall).__thash_h_ M(Syscall)._thash_h.
+            wp; sp.
+            exists * node0{2}, node1{2}, pub_seed1{1}, addr0{1}, address{2} .
+            elim * => P0 P1 P2 P3 P4.
+            call (rand_hash_results P0 P1 P2 P3 P4) => [/# |].
+            auto => /> &1 &2 H0 H1 H2 H3 H4 H5 H6 H7 H8 H9 H10 H11 H12 H13 H14 H15 H16 H17 H18 H19 H20 H21 H22 H23 H24 H25 H26 H27 H28.
+            do split.
+              - smt(merge_nbytes_val).
+              - smt(sub_k).
+              - move => H29 H30 resultL resultR H31 H32.
+                do split; [| smt() | smt() |]; (
+                     apply (eq_from_nth witness); [by rewrite !size_sub | rewrite size_sub // => i?];
+                    rewrite !nth_sub //=/#
+                ).
 
+ecall {1} (p_treehash_condition_correct_eq heights{1} offset{1}).
+wp.
+ecall {1} (memcpy_u8u8_3_352_32_post _stack{1} buf{1} t64{1}).
+auto => /> &1 &2 H0 H1 H2 H3 H4 H5 H6 H7 H8 H9 H10 H11 H12 H13 H14 H15 H16 H17 H18 H19 H20 H21 H22 H23 H24 H25 H26 H27 H28 H29. 
+do split; 1,2: by rewrite to_uintM of_uintK /= to_uintB; [by rewrite uleE /# | by rewrite of_uintK /= /#].
+move => H30 H31 resultStack H32 H33 H34*.
+do split; 1,2: by rewrite to_uintB 2:/# uleE /#.
+rewrite !size_put.
+have ->: to_uint (offset{1} - W64.one) = to_uint offset{1} - 1 by rewrite to_uintB // uleE /#.
+move  => ?? result_cond Hcond. 
+have E1: forall (k : int), 0 <= k < to_uint offset{1} => to_uint heights{1}.[k] = nth witness heights{2} k.
+   + move => k?.
+     have ->: nth witness heights{2} k = nth witness (sub_list heights{2} 0 (to_uint offset{1})) k by rewrite /sub_list nth_mkseq /#.
+     rewrite -H17 (nth_map witness); [by rewrite size_sub /# | by rewrite nth_sub /#].
+have E2: forall (k : int), 0 <= k < to_uint offset{1} => 0 <= to_uint heights{1}.[k] < XMSS_TREE_HEIGHT by smt().         
+do split => //; 1,6,7: by smt(). (* trivial solves two goals: 12 vs 10 subgoals *)
+   + apply (eq_from_nth witness); first by rewrite size_map size_sub_list 1:/# size_sub /#. 
+     rewrite size_map size_sub 1:/# => i?.
+     rewrite /sub_list nth_mkseq 1:/# /= nth_put 1:/#.
+     rewrite (nth_map witness); first by rewrite size_sub /#.     
+     rewrite nth_sub 1:/# /= get_setE.
+       * rewrite to_uintB; first by rewrite uleE to_uintB 2:/# uleE /#.
+         rewrite /= to_uintB 2:/# uleE /#.
+     case (i = to_uint offset{1} - 2) => [-> |?].
+       * rewrite ifT; first by rewrite to_uintB; [by rewrite uleE to_uintB 2:/# uleE /# | by rewrite /= to_uintB 2:/# uleE /#].
+         have ->: to_uint (offset{1} - W64.one - W64.one) = to_uint offset{1} - 2 by rewrite to_uintB; [by rewrite uleE to_uintB 2:/# uleE /# | by rewrite /= to_uintB 2:/# uleE /#].
+         rewrite ifT // to_uintD_small 1:/# E1 /#.
+       * have ->: to_uint (offset{1} - W64.one - W64.one) = to_uint offset{1} - 2 by rewrite to_uintB; [by rewrite uleE to_uintB 2:/# uleE /# | by rewrite /= to_uintB 2:/# uleE /#].
+         rewrite ifF 1:/# ifF 1:/# /#.
+   + move => k??.     
+     split; [rewrite nth_put /# |]. 
+     rewrite !nth_put 1:/#.
+     case (k = to_uint offset{1} - 2) => H; last by rewrite ifF /#.
+     rewrite ifT 1:/# => ?.
+     admit. (* Range das heights *)
+
+   + apply (eq_from_nth witness); first by rewrite size_sub 1:/# size_sub_list /#.
+     rewrite size_sub 1:/# => j?.
+     rewrite nth_sub 1:/# /= /sub_list nth_mkseq 1:/# /= nth_nbytes_flatten; first by rewrite size_put /#.
+     rewrite nth_put 1:/#.
+     move: H32 H33 H34.
+     have ->: to_uint ((offset{1} - (of_int 2)%W64) * (of_int 32)%W64) = (to_uint offset{1} - 2) * 32.
+       * rewrite to_uintM of_uintK /=.
+         rewrite to_uintB; first by rewrite uleE /#.
+         rewrite of_uintK /#.
+     move => H32 H33 H34.
+     case (to_uint offset{1} - 2 = j %/ n) => H.
+       * rewrite -H29 get_to_list -H33 /#. 
+       * rewrite H32 1:/#.
+         have ->: _stack{1}.[j] = nth witness (sub _stack{1} 0 (n * to_uint offset{1})) j by rewrite nth_sub /#.
+         by rewrite H19 /sub_list nth_mkseq 1:/# /= nth_nbytes_flatten 1:/#.
+   + rewrite Hcond /treehash_cond.
+     have ->: to_uint (offset{1} - W64.one - W64.one) = to_uint offset{1} - 2 by rewrite to_uintB; [by rewrite uleE to_uintB 2:/# uleE /# | by rewrite /= to_uintB 2:/# uleE /#].
+     have ->: to_uint (offset{1} - W64.one) = to_uint offset{1} - 1 by rewrite to_uintB 2:/# uleE /#.
+     reflexivity.
+   + have E21: (2 <= to_uint offset{1} /\heights{1}.[to_uint offset{1} - 2] = heights{1}.[to_uint offset{1} - 1]) by smt().
+     move: E21 => [#] Ha Hb.
+      admit. (* 2 <= to_uint offset{1} - 1 *)
+   + rewrite !nth_put 1,2:/# ifT // ifF 1:/#. 
+     move: Hcond. 
+     have ->: to_uint (offset{1} - W64.one - W64.one) = to_uint offset{1} - 2 by rewrite to_uintB; [by rewrite uleE to_uintB 2:/# uleE /# | by rewrite /= to_uintB 2:/# uleE /#].
+     rewrite /treehash_cond.
+     have ->: to_uint (offset{1} - W64.one) = to_uint offset{1} - 1 by rewrite to_uintB 2:/# uleE /#.
+     have E21: (2 <= to_uint offset{1} /\heights{1}.[to_uint offset{1} - 2] = heights{1}.[to_uint offset{1} - 1]) by smt().
+     move: E21 => [Ha Hb].
+     rewrite !get_setE 1,2:/# ifF 1:/# ifT 1:/# /=.
+     move => Hcond.
+     rewrite -E1 1:/#. 
+
+     
+     rewrite Hb. rewrite to_uintK.
+     rewrite E1 1:/#.
+
+     admit.
+   + move => Ha.
+     rewrite !nth_put 1,2:/# ifT // ifF 1:/#.
+     rewrite -!E1 1,2:/# => Hb.
+     rewrite Hcond /treehash_cond.
+     do split; first by smt(@W64 pow2_64).
+     have ->: to_uint (offset{1} - W64.one - W64.one) = to_uint offset{1} - 2 by rewrite to_uintB; [by rewrite uleE to_uintB 2:/# uleE /# | by rewrite /= to_uintB 2:/# uleE /#].
+     have ->: to_uint (offset{1} - W64.one) = to_uint offset{1} - 1 by rewrite to_uintB 2:/# uleE /#.
+     rewrite !get_setE 1,2:/# /= ifF 1:/#. 
+     have ->: heights{1}.[to_uint offset{1} - 3] = W32.of_int (to_uint  heights{1}.[to_uint offset{1} - 3]) by rewrite to_uintK.
+     have ->: heights{1}.[to_uint offset{1} - 2] + W32.one = W32.of_int (to_uint heights{1}.[to_uint offset{1} - 2] + 1) by smt(@W32 pow2_32).
+     by rewrite !Hb.
+qed.
