proof/correctness/test.ec
@@ -1,6 +1,0 @@
-require import AllCore.
-
-lemma test : forall x y, x + 2 * y <= 4 && 2 * x + y <= 4 => x + y < 3.
-proof.
-coq edit "test" ().
-qed.
