test/address_properties/README.md
@@ -1,23 +1,11 @@
 # Address
 
-```
-==============================================================
-[gen chain inplace:]
-index 6 was changed: value = 9 // MIN (start + steps - 1, w - 1)
-index 7 was changed: value = 1
-==============================================================
+## `#pre`
 
 ```
-
-```
-[expand_seed]: Changing index 5 of the address does not change the result
-[expand_seed]: Changing index 6 of the address does not change the result
-[expand_seed]: Changing index 7 of the address does not change the result
-
-[expand seed:]
-index 5 was changed: value = 66 // len - 1
-index 6 was changed: value = 0
-index 7 was changed: value = 0
+[wots_pkgen]: Changing index 5 of the address does not change the result
+[wots_pkgen]: Changing index 6 of the address does not change the result
+[wots_pkgen]: Changing index 7 of the address does not change the result
 ```
 
 ```
@@ -29,7 +17,18 @@ index 7 was changed: value = 0
 [l_tree]: Changing index 5 of the address changes the result
 [l_tree]: Changing index 6 of the address changes the result
 [l_tree]: Changing index 7 of the address changes the result
-[l_tree:] index 5 was changed: value = 7
+```
+
+## `#post`
+
+```
+[wots pk gen:] index 5 was changed: value = 66
+[wots pk gen:] index 6 was changed: value = 14
+[wots pk gen:] index 7 was changed: value = 1
+```
+
+```
+[l_tree:] index 5 w as changed: value = 7
 [l_tree:] index 6 was changed: value = 0
 [l_tree:] index 7 was changed: value = 2
 ```
